Vir/React/Core.lean
@@ -36,9 +36,8 @@ end ElementType
 /-- Creates a native function component from a Lean render callback. -/
 def FunctionComponent.ofLean
     (render : Lean.Vir.Js props → ReactM (Lean.Vir.Js Node)) :
-    Lean.Vir.RuntimeM (FunctionComponent props) := by
-  unfold ReactM at render
-  exact Lean.Vir.Js.Function.ofLean render
+    Lean.Vir.RuntimeM (FunctionComponent props) :=
+  Lean.Vir.Js.Function.ofLean render
 
 namespace Node
 
